-

Formula.v
@@ -2269,6 +2269,31 @@ Fixpoint Nat_pow_mod_loop a b c :=
   end.
 
 Definition Nat_pow_mod a b c := Nat_pow_mod_loop a b c.
+Definition inv_mod i n := Nat_pow_mod i (n - 2) n.
+
+(* *)
+
+Theorem Nat_pow_mod_is_pow_mod : ∀ a b c,
+  c ≠ 0 → Nat_pow_mod a b c = (a ^ b) mod c.
+Proof.
+intros * Hcz.
+destruct (le_dec c 1) as [Hc1 | Hc1]. {
+  unfold Nat_pow_mod.
+  destruct c; [ easy | ].
+    destruct b.
+cbn.
+...
+revert a c.
+induction b; intros. {
+  cbn. rewrite Nat.mod_small.
+...
+
+Theorem inv_mod_neq : ∀ i p,
+  is_prime p = true → 2 ≤ i ≤ p - 2 → inv_mod i p ≠ i.
+Proof.
+intros * Hp Hip Hcon.
+unfold inv_mod in Hcon.
+...
 
 (* from a prime number p, group together values "a" between 2 and
    p-2 with their inverse modulo p, which is "a^(p-2)" according
